Making transition to De Bruijn indices

Nederpelt/Lambda2.lean
@@ -1,28 +1,10 @@
 import Mathlib.Data.Finset.Basic
 
-
 inductive 𝕋2 (𝕍 : Type) : Type
 | TVar : 𝕍    → 𝕋2 𝕍
 | To   : 𝕋2 𝕍 → 𝕋2 𝕍 → 𝕋2 𝕍
 | TTo  : 𝕍 → 𝕋2 𝕍 → 𝕋2 𝕍
 deriving DecidableEq
-
-@[simp]
-def substTVar {𝕍 : Type} [DecidableEq 𝕍] (α : 𝕍) (σ : 𝕋2 𝕍) : 𝕋2 𝕍 → 𝕋2 𝕍
-| .TVar α' => 
-  if α = α'
-  then σ
-  else .TVar α'
-| .To τ τ' => .To (substTVar α σ τ) (substTVar α σ τ')
-| .TTo α' τ => 
-  .TTo α' (if α = α' then σ else (substTVar α σ τ))
-
-
-@[simp]
-def freeTVarsOfType {𝕍 : Type} [DecidableEq 𝕍] : 𝕋2 𝕍 → Finset 𝕍
-| (.TVar α) => {α}
-| (.To σ₁ σ₂) => (freeTVarsOfType σ₁) ∪ (freeTVarsOfType σ₂)
-| (.TTo α σ) => (freeTVarsOfType σ).erase α
 
 inductive Λ2 (V : Type) (𝕍 : Type) : Type
 | Var  : V → Λ2 V 𝕍
@@ -31,8 +13,40 @@ inductive Λ2 (V : Type) (𝕍 : Type) : Type
 | Lam  : V → 𝕋2 𝕍 → Λ2 V 𝕍 → Λ2 V 𝕍
 | TLam : 𝕍 → Λ2 V 𝕍 → Λ2 V 𝕍
 
+inductive TCtxt2 (V : Type) (𝕍 : Type) : Type
+| Empty       : TCtxt2 V 𝕍
+| TypeVarCtxt : 𝕍 → TCtxt2 V 𝕍 → TCtxt2 V 𝕍
+| VarCtxt     : V → 𝕋2 𝕍 → TCtxt2 V 𝕍 → TCtxt2 V 𝕍  
+
+notation:9 σ " →' " τ => 𝕋2.To σ τ 
+notation:9 Γ ";; " x " : " σ => TCtxt2.VarCtxt x σ Γ
+notation:9 Γ ";; " α " : * " => TCtxt2.TypeVarCtxt α Γ
+notation:9 "Π " α " : *, " σ => 𝕋2.TTo α σ
+notation:9 "λ' " x " : " σ ", " M => Λ2.Lam x σ M
+notation:9 "λ' " α " : *, " M => Λ2.TLam α M
+notation:9 M " ⟪" σ "⟫" => Λ2.TApp M σ
+
+variable {V 𝕍 : Type}
+variable [DecidableEq V] [DecidableEq 𝕍] 
+
 @[simp]
-def freeVarsOfTerm {V 𝕍 : Type} [DecidableEq V] : Λ2 V 𝕍 → Finset V
+def subTVarInType (α : 𝕍) (σ : 𝕋2 𝕍) : 𝕋2 𝕍 → 𝕋2 𝕍
+| .TVar α' => 
+  if α = α'
+  then σ
+  else .TVar α'
+| .To τ τ' => .To (subTVarInType α σ τ) (subTVarInType α σ τ')
+| .TTo α' τ => 
+  .TTo α' (if α = α' then σ else (subTVarInType α σ τ))
+
+@[simp]
+def freeTVarsOfType : 𝕋2 𝕍 → Finset 𝕍
+| (.TVar α) => {α}
+| (.To σ₁ σ₂) => (freeTVarsOfType σ₁) ∪ (freeTVarsOfType σ₂)
+| (.TTo α σ) => (freeTVarsOfType σ).erase α
+
+@[simp]
+def freeVarsOfTerm : Λ2 V 𝕍 → Finset V
 | .Var x     => {x}
 | .App M N   => (freeVarsOfTerm M) ∪ (freeVarsOfTerm N)
 | .TApp M _  => freeVarsOfTerm M
@@ -40,32 +54,47 @@ def freeVarsOfTerm {V 𝕍 : Type} [DecidableEq V] : Λ2 V 𝕍 → Finset V
 | .TLam _ M  => freeVarsOfTerm M
 
 @[simp]
-def freeTVarsOfTerm {V 𝕍 : Type} [DecidableEq 𝕍] : Λ2 V 𝕍 → Finset 𝕍
+def freeTVarsOfTerm : Λ2 V 𝕍 → Finset 𝕍
 | .Var  _     => {}
 | .App  M N   => (freeTVarsOfTerm M) ∪ (freeTVarsOfTerm N)
 | .TApp M σ   => (freeTVarsOfTerm M) ∪ (freeTVarsOfType σ)
 | .Lam  _ σ M => (freeTVarsOfTerm M) ∪ (freeTVarsOfType σ)
 | .TLam α M   => (freeTVarsOfTerm M).erase α
 
-inductive TCtxt2 (V : Type) (𝕍 : Type) : Type
-| Empty       : TCtxt2 V 𝕍
-| TypeVarCtxt : 𝕍 → TCtxt2 V 𝕍 → TCtxt2 V 𝕍
-| VarCtxt     : V → 𝕋2 𝕍 → TCtxt2 V 𝕍 → TCtxt2 V 𝕍   
+@[simp]
+def subVarInTerm (x : V) (N : Λ2 V 𝕍) : Λ2 V 𝕍 → Λ2 V 𝕍
+| .Var x'     => if x = x'
+                 then N 
+                 else Λ2.Var x'
+| .App M M'   => Λ2.App (subVarInTerm x N M) (subVarInTerm x N M')
+| .TApp M τ   => Λ2.TApp (subVarInTerm x N M) τ
+| .Lam x' τ M => Λ2.Lam x' τ (if x = x' then M else subVarInTerm x N M)
+| .TLam α M   => Λ2.TLam α (subVarInTerm x N M)
 
 @[simp]
-def TDomTCtxt {V 𝕍 : Type} [DecidableEq 𝕍] : TCtxt2 V 𝕍 → Finset 𝕍
+def subTVarInTerm (α : 𝕍) (σ : 𝕋2 𝕍) : Λ2 V 𝕍 → Λ2 V 𝕍
+| .Var x'     => Λ2.Var x'
+| .App M M'   => Λ2.App (subTVarInTerm α σ M) (subTVarInTerm α σ M')
+| .TApp M τ   => Λ2.TApp (subTVarInTerm α σ M) (subTVarInType α σ τ)
+| .Lam x' τ M => Λ2.Lam x' (subTVarInType α σ τ) (subTVarInTerm α σ M)
+| .TLam α' M   => if α = α'
+                  then Λ2.TLam α' M
+                  else Λ2.TLam α' (subTVarInTerm α σ M) 
+
+@[simp]
+def TDomTCtxt : TCtxt2 V 𝕍 → Finset 𝕍
 | .Empty           => {} 
 | .TypeVarCtxt α Γ => {α} ∪ (TDomTCtxt Γ)
 | .VarCtxt _ _ Γ   => TDomTCtxt Γ
 
 @[simp]
-def DomTCtxt {V 𝕍 : Type} [DecidableEq V] : TCtxt2 V 𝕍 → Finset V
+def DomTCtxt : TCtxt2 V 𝕍 → Finset V
 | .Empty           => {} 
 | .TypeVarCtxt _ Γ => DomTCtxt Γ
 | .VarCtxt x _ Γ   => (DomTCtxt Γ) ∪ {x}
 
 @[simp]
-def getType {V 𝕍 : Type} [DecidableEq V] (x : V) : TCtxt2 V 𝕍 → Option (𝕋2 𝕍)
+def getType (x : V) : TCtxt2 V 𝕍 → Option (𝕋2 𝕍)
 | .Empty => none
 | .TypeVarCtxt _ Γ => getType x Γ 
 | .VarCtxt x' σ Γ => 
@@ -73,10 +102,27 @@ def getType {V 𝕍 : Type} [DecidableEq V] (x : V) : TCtxt2 V 𝕍 → Option (
     then some σ
     else getType x Γ
 
-lemma typeOfDefinedOfInTCtxt {V 𝕍 : Type} [DecidableEq V] : 
+lemma getTypeRebind {Γ : TCtxt2 V 𝕍} {y : V} {σ σ' : 𝕋2 𝕍} :
+    ∀ x : V, getType x ((Γ;; y : σ);; y : σ') = getType x (Γ;; y : σ') := by
+  introv; simp; split_ifs <;> rfl
+
+lemma getTypeReorder {Γ : TCtxt2 V 𝕍} {x y : V} {σ σ' : 𝕋2 𝕍} :
+    x ≠ y → 
+      ∀ {z : V}, getType z ((Γ;;x : σ);; y : σ') = getType z ((Γ;;y : σ');; x : σ) := by
+  intro h z
+  by_cases h' : z = x
+  · simp [h, h']
+  · by_cases h'' : z = y
+    · simp [h', h'']
+      split_ifs with h
+      · exfalso; rw [h''] at h'; exact h' h 
+      · rfl;
+    · simp [h', h'']
+
+lemma typeOfDefinedOfInTCtxt : 
   ∀ (Γ : TCtxt2 V 𝕍) (x : V), 
     x ∈ DomTCtxt Γ → (∃ σ : 𝕋2 𝕍, (getType x Γ) = (some σ)) := by
-  intros Γ x;
+  intros Γ x
   induction' Γ with α Γ h_ind x' σ Γ h_ind
   · simp
   · simp only [DomTCtxt, getType]; assumption
@@ -85,7 +131,7 @@ lemma typeOfDefinedOfInTCtxt {V 𝕍 : Type} [DecidableEq V] :
     · simp [h']
     · simp only [h', or_false, ite_false]; assumption
 
-def wellFormedTCtxt {V 𝕍 : Type} [DecidableEq V] [DecidableEq 𝕍] : TCtxt2 V 𝕍 → Prop 
+def wellFormedTCtxt : TCtxt2 V 𝕍 → Prop 
 | .Empty => True
 | .TypeVarCtxt α Γ => α ∉ TDomTCtxt Γ ∧ wellFormedTCtxt Γ
 | .VarCtxt x σ Γ => x ∉ DomTCtxt Γ ∧ 
@@ -95,7 +141,7 @@ def wellFormedTCtxt {V 𝕍 : Type} [DecidableEq V] [DecidableEq 𝕍] : TCtxt2 
                     wellFormedTCtxt Γ
 
 @[simp]
-def typeOf {V 𝕍 : Type} [DecidableEq V] [DecidableEq 𝕍] (Γ : TCtxt2 V 𝕍) : Λ2 V 𝕍 → Option (𝕋2 𝕍)
+def typeOf (Γ : TCtxt2 V 𝕍) : Λ2 V 𝕍 → Option (𝕋2 𝕍)
 | .Var x => getType x Γ
 | .App M N => 
   match typeOf Γ M with
@@ -106,7 +152,7 @@ def typeOf {V 𝕍 : Type} [DecidableEq V] [DecidableEq 𝕍] (Γ : TCtxt2 V �
   | _               => none
 | .TApp M σ => 
   match typeOf Γ M with
-  | .some (.TTo α τ) => some (substTVar α σ τ)
+  | .some (.TTo α τ) => some (subTVarInType α σ τ)
   | _                => none
 | .Lam x σ M => 
   match typeOf (.VarCtxt x σ Γ) M with 
@@ -117,47 +163,253 @@ def typeOf {V 𝕍 : Type} [DecidableEq V] [DecidableEq 𝕍] (Γ : TCtxt2 V �
   | .some τ => some (.TTo α τ)
   | _       => none
 
+lemma ctxtTypeOfPreservation {M : Λ2 V 𝕍} : 
+  ∀ {Γ Γ': TCtxt2 V 𝕍},
+    (∀ x : V, x ∈ freeVarsOfTerm M → getType x Γ = getType x Γ') → 
+      typeOf Γ M = typeOf Γ' M := by
+  induction M with
+  | Var x => intro Γ Γ' h; apply h; simp
+  | App M N ih₁ ih₂ =>
+    intro Γ Γ' h
+    have h₁ (x : V) (h' : x ∈ freeVarsOfTerm M) : getType x Γ = getType x Γ' := by
+      exact h x (by simp only [freeVarsOfTerm, Finset.mem_union, h', true_or])
+    have h₂ (x : V) (h' : x ∈ freeVarsOfTerm N) : getType x Γ = getType x Γ' := by
+      exact h x (by simp only [freeVarsOfTerm, Finset.mem_union, h', or_true])
+    simp [ih₁ h₁, ih₂ h₂]
+  | TApp M σ ih => intro Γ Γ' h; simp [ih h]
+  | Lam y σ M ih => 
+    intro Γ Γ' h
+    have h (x : V) (h' : x ∈ freeVarsOfTerm M) : getType x (Γ;; y : σ) = getType x (Γ';; y : σ) := by
+      by_cases h'' : x = y <;> simp[h'']
+      exact h x (Finset.mem_erase_of_ne_of_mem h'' h')
+    simp [ih h]
+  | TLam α M ih =>
+    intro Γ Γ' h
+    have h (x : V) (h' : x ∈ freeVarsOfTerm M) : 
+      getType x (Γ;; α : * ) = getType x (Γ';; α : * ) := by simp [h x h']
+    simp [ih h]
+
 @[simp]
-def typingJudgement {V 𝕍 : Type} [DecidableEq V] [DecidableEq 𝕍] 
+def typingJudgement
     (Γ : TCtxt2 V 𝕍) (M : Λ2 V 𝕍) (σ : 𝕋2 𝕍) : Prop :=
   typeOf Γ M = some σ
 
-def formationRule {V 𝕍 : Type} [DecidableEq 𝕍] (Γ : TCtxt2 V 𝕍) (σ : 𝕋2 𝕍) : Prop := freeTVarsOfType σ ⊆ TDomTCtxt Γ
+def formationRule (Γ : TCtxt2 V 𝕍) (σ : 𝕋2 𝕍) : Prop := 
+  freeTVarsOfType σ ⊆ TDomTCtxt Γ
 
 notation:10 Γ " ⊢ " M " : " σ => typingJudgement Γ M σ
 notation:10 Γ " ⊢ " σ " : * " => formationRule Γ σ
-notation:9 σ " →' " τ => 𝕋2.To σ τ 
-notation:9 Γ ";; " x " : " σ => TCtxt2.VarCtxt x σ Γ
-notation:9 Γ ";; " α " : * " => TCtxt2.TypeVarCtxt α Γ
-notation:9 "Π " α " : *, " σ => 𝕋2.TTo α σ
-notation:9 "λ' " x " : " σ ", " M => Λ2.Lam x σ M
-notation:9 "λ' " α " : *, " M => Λ2.TLam α M
-notation:9 M " ⟪" σ "⟫" => Λ2.TApp M σ
 
-instance {V 𝕍: Type} : Coe V (Λ2 V 𝕍) where
+@[simp]
+lemma unfoldTypingJudgement {Γ : TCtxt2 V 𝕍} {M : Λ2 V 𝕍} {σ : 𝕋2 𝕍} :
+  (Γ ⊢ M : σ) → (typeOf Γ M = some σ) := id
+
+instance : Coe V (Λ2 V 𝕍) where
   coe := .Var 
-instance {V 𝕍 : Type} : CoeFun (Λ2 V 𝕍) (fun _ => Λ2 V 𝕍 → Λ2 V 𝕍) where
+instance : CoeFun (Λ2 V 𝕍) (fun _ => Λ2 V 𝕍 → Λ2 V 𝕍) where
   coe := .App 
 
-lemma var_rule {V 𝕍 : Type} [DecidableEq V] [DecidableEq 𝕍] (Γ : TCtxt2 V 𝕍) (x : V) (σ : 𝕋2 𝕍) :
+lemma var_rule (Γ : TCtxt2 V 𝕍) (x : V) (σ : 𝕋2 𝕍) :
   getType x Γ = some σ → (Γ ⊢ x : σ) := by simp
 
-lemma appl_rule {V 𝕍 : Type} [DecidableEq V] [DecidableEq 𝕍] (Γ : TCtxt2 V 𝕍) (M N : Λ2 V 𝕍) (σ τ : 𝕋2 𝕍) : 
-  (Γ ⊢ M : σ →' τ) → (Γ ⊢ N : σ) → (Γ ⊢ M N : τ) := by
-    intros h h'; unfold typingJudgement at *; simp [h, h']
+lemma appl_rule (Γ : TCtxt2 V 𝕍) (M N : Λ2 V 𝕍) (τ : 𝕋2 𝕍) : 
+  (∃ σ, (Γ ⊢ M : σ →' τ) ∧ (Γ ⊢ N : σ)) ↔ (Γ ⊢ M N : τ) := by
+    apply Iff.intro
+    · rintro ⟨σ, h, h'⟩; unfold typingJudgement at *; simp [h, h']
+    · intro h
+      simp only [typingJudgement, typeOf] at h 
+      generalize h' : typeOf Γ M = x; rw [h'] at h
+      match x with
+        | none => simp at h
+        | some val => 
+          match val with
+          | .To σ τ' => 
+            use σ
+            simp only at h 
+            split_ifs at h with h''
+            simp only [Option.some.injEq] at h 
+            rw [h] at h'
+            exact ⟨h', h''⟩
 
-lemma abst_rule {V 𝕍 : Type} [DecidableEq V] [DecidableEq 𝕍] (Γ : TCtxt2 V 𝕍) (M : Λ2 V 𝕍) (x : V) (σ τ : 𝕋2 𝕍) :
+lemma abst_rule (Γ : TCtxt2 V 𝕍) (M : Λ2 V 𝕍) (x : V) (σ τ : 𝕋2 𝕍) :
   ((Γ;; x : σ) ⊢ M : τ) → (Γ ⊢ (λ' x : σ, M) : σ →' τ) := by
     intros h; unfold typingJudgement at *; simp [h]
 
-lemma appl₂_rule {V 𝕍 : Type} [DecidableEq V] [DecidableEq 𝕍] (Γ : TCtxt2 V 𝕍) (α : 𝕍) (M : Λ2 V 𝕍) (σ τ : 𝕋2 𝕍) :
-  (Γ ⊢ M : Π α : *, σ) → (Γ ⊢ σ : *) → (Γ ⊢ M ⟪τ⟫ : substTVar α τ σ) := by
+lemma appl₂_rule (Γ : TCtxt2 V 𝕍) (α : 𝕍) (M : Λ2 V 𝕍) (σ τ : 𝕋2 𝕍) :
+  (Γ ⊢ M : Π α : *, σ) → (Γ ⊢ σ : *) → (Γ ⊢ M ⟪τ⟫ : subTVarInType α τ σ) := by
     intros h _; simp only [typingJudgement, typeOf] at *; simp [h]
 
-lemma abst₂_rule {V 𝕍 : Type} [DecidableEq V] [DecidableEq 𝕍] (Γ : TCtxt2 V 𝕍) (α : 𝕍) (M : Λ2 V 𝕍) (σ : 𝕋2 𝕍) :
+lemma abst₂_rule (Γ : TCtxt2 V 𝕍) (α : 𝕍) (M : Λ2 V 𝕍) (σ : 𝕋2 𝕍) :
   ((Γ;; α : *) ⊢ M : σ) → (Γ ⊢ (λ' α : *, M) : (Π α : *, σ)) := by
     intros h; unfold typingJudgement at h; simp [h]
 
-
+lemma typeUniqueness (Γ : TCtxt2 V 𝕍) (M : Λ2 V 𝕍) (σ τ : 𝕋2 𝕍) :
+  (Γ ⊢ M : σ) → (Γ ⊢ M : τ) → σ = τ := by
+    intros h h'; unfold typingJudgement at *; rw [h, Option.some.injEq] at h'; assumption
   
+def lambda2BetaReduction : Λ2 V 𝕍 → Λ2 V 𝕍 → Prop
+| .Lam x σ M, R => ∃ M', R = Λ2.Lam x σ M' ∧ lambda2BetaReduction M M'
+| .TLam α M, R  => ∃ M', R = Λ2.TLam α M' ∧ lambda2BetaReduction M M'
+| .App M N, R => 
+    (∃ M' N' : Λ2 V 𝕍, R = M' N' ∧
+      (
+        (lambda2BetaReduction M M' ∧ N' = N) ∨
+        (lambda2BetaReduction N N' ∧ M' = M)
+      )
+    ) ∨
+    (
+      match M with
+      | .Lam x σ M' => R = subVarInTerm x N M'
+      | _           => False
+    ) 
+| .TApp M σ, R => 
+  (∃ M', R = Λ2.TApp M' σ ∧ lambda2BetaReduction M M') ∨
+  (
+    match M with
+    | .TLam α M' => R = subTVarInTerm α σ M' 
+    | _          => False
+  )
+| .Var _, _ => False
 
+lemma varSubPreservesTypeVar 
+  {Γ : TCtxt2 V 𝕍} {N : Λ2 V 𝕍} {x y : V} {σ : 𝕋2 𝕍} : (Γ ⊢ N : σ) →
+    typeOf (Γ;; x : σ) (Λ2.Var y) = typeOf Γ (subVarInTerm x N (Λ2.Var y)) := by
+  intro h
+  simp
+  split_ifs with h' h'' h''
+  · rw [h]
+  · exfalso; exact h'' (Eq.symm h')
+  · exfalso; exact h' (Eq.symm h'')
+  · simp
+
+lemma varSubPreservesType {M N : Λ2 V 𝕍} {x : V} {σ : 𝕋2 𝕍} :
+    ∀ {Γ : TCtxt2 V 𝕍}, (Γ ⊢ N : σ) → typeOf (Γ;; x : σ) M = typeOf Γ (subVarInTerm x N M) := by
+  intros Γ h
+  induction M with
+  | Var y => exact varSubPreservesTypeVar h
+  | App _ _ ih₁ ih₂ => simp [ih₁, ih₂]
+  | TApp M τ ih => simp [ih]
+  | Lam y τ M ih =>
+    by_cases h' : x = y
+    · simp [h']
+      rw [ctxtTypeOfPreservation]
+      intros x _
+      exact getTypeRebind x
+    · simp [h']
+      
+
+      
+
+
+
+
+
+
+
+    
+    
+
+
+
+
+
+   
+-- lemma varSubPreservesType {V 𝕍 : Type} [DecidableEq V] [DecidableEq 𝕍] (Γ : TCtxt2 V 𝕍) (M N : Λ2 V 𝕍) (x : V) (σ τ : 𝕋2 𝕍) :
+--   (Γ ⊢ (λ' x : τ, M) N : σ) → (Γ ⊢ (subVarInTerm x N M) : σ) := by
+--     intros h
+--     rw [←appl_rule] at h
+--     rcases h with ⟨τ', h₁, h₂⟩
+--     simp at h₁
+--     generalize h : typeOf (Γ;; x : τ) M = σM
+--     rw [h] at h₁
+--     match σM with
+--     | none => simp at h₁
+--     | some σ' => 
+--       simp at h₁
+--       rw [←h₁.1] at h₂
+--       rw [h₁.2] at h
+--       clear h₁
+--       revert σ
+--       revert Γ
+--       induction M with
+--       | Var y => 
+--         intros Γ h₂ σ h₁; exact varSubPreservesTypeVar σ h₁ h₂
+--       | App M₁ M₂ ih₁ ih₂ => 
+--         intros Γ h₂ σ h₁
+--         simp at h₁
+--         generalize aux : typeOf (Γ;; x : τ) M₁ = σM₁
+--         rw [aux] at h₁
+--         match σM₁ with
+--         | some (.To τ' σ') => 
+--           simp at h₁
+--           split_ifs at h₁ with aux'
+--           · rw [Option.some.injEq] at h₁ 
+--             rw [h₁] at aux
+--             specialize ih₁ Γ h₂ (τ' →' σ) aux
+--             specialize ih₂ Γ h₂ τ' aux'
+--             simp at ih₁ ih₂
+--             simp
+--             rw [ih₁, ih₂]
+--             simp
+--       | TApp M γ ih => 
+--         intros Γ h₂ σ h₁
+--         simp at h₁
+--         generalize aux : typeOf (Γ;; x : τ) M = σM
+--         rw [aux] at h₁
+--         match σM with
+--         | some (Π α : *, τ') => 
+--           simp at h₁
+--           specialize ih Γ h₂ (Π α : *, τ') aux
+--           simp at ih
+--           simp [ih, h₁]
+--         | some (.TVar x) => simp at h₁
+--         | some (_ →' _) =>  simp at h₁
+--         | none => simp at h₁ 
+--       | Lam y σ' M ih =>
+--         intros Γ h₂ σ h₁
+--         simp at h₁
+--         unfold subVarInTerm
+--         split_ifs with cond
+--         · simp [cond] at h₁
+--           simp [←h₁, ctxtTypeOfPreservation (λ _ _ => getTypeRebind)]
+--         · simp -- [←h₁]
+--           have h' : 
+--               ∀ (z : V), z ∈ freeVarsOfTerm M →
+--                 getType z ((Γ;; x : τ);; y : σ') = getType z ((Γ;; y : σ');; x : τ) := 
+--             λ _ _ => getTypeReorder cond
+--           rw [ctxtTypeOfPreservation h'] at h₁
+
+--           specialize ih (Γ;; y : σ') 
+          
+
+
+
+
+
+            
+
+--           specialize ih (Γ;; y : σ') 
+
+
+          
+          
+
+          
+
+
+--       | TLam α M => sorry
+
+
+
+
+
+
+
+
+
+
+
+
+
+
+notation:9 M "→ᵦ" N => lambda2BetaReduction M N 
